src/vminus/CompilerTestAnswers.v
@@ -1,0 +1,223 @@
+Require Import List.
+Import ListNotations.
+Require Import String.
+Require Import Arith.
+
+Require Import QuickChick.QuickChick.
+Import QcDefaultNotation. Open Scope qc_scope.
+
+Require Import Vminus.Vminus.
+Require Import Vminus.Atom.
+Require Import Vminus.ListCFG.
+Require Import Vminus.Imp.
+Require Import Vminus.Compiler.
+Require Import Vminus.CompilerProp.
+
+Require Import Vminus.ImpGen.
+Require Import Vminus.VminusGen.
+Require Import Vminus.CompilerGen.
+
+Require Import Vminus.CompilerTest.
+
+(**! Section test_compile_bexp extends compiler *)
+
+(* Fatal error with stack overflow 
+Definition comp_bop_correct_checker: Checker :=
+  forAll arbitrary (fun (a1: aexp) =>
+  forAll arbitrary (fun (a2: aexp) =>
+  forAll arbitrary (fun (binop: bop) => 
+    collect (binop, a1, a2) (comp_correct_checker 
+      (comp_bop binop (comp_aexp a1) (comp_aexp a2))
+      (fun m => V.Opsem.bop_denote binop (aeval a1 m) (aeval a2 m)))))).
+ *)
+
+Definition comp_bop_correct_checker: Checker :=
+  forAll arbitrary (fun (a1: aexp) =>
+  forAll arbitrary (fun (a2: aexp) =>
+  forAll arbitrary (fun (binop: bop) => 
+    collect binop (comp_correct_checker 
+      (comp_bop binop (comp_aexp a1) (comp_aexp a2))
+      (fun m => V.Opsem.bop_denote binop (aeval a1 m) (aeval a2 m)))))).
+
+(*! QuickChick comp_bop_correct_checker. *)
+
+
+Definition comp_bexp_correct_checker : Checker :=
+  forAll arbitrary (fun b: bexp => 
+    comp_correct_checker (comp_bexp b) (fun m => if (beval b m) then 1 else 0)).
+
+(* QuickChick comp_bexp_correct_checker. *)
+
+(** Exercise: Now write a checker for the following.
+
+Lemma comp_store_correct : 
+  forall g a v le lr cs st,
+  insns_at_pc g (block_entry le) (steval (comp_store a v lr) cs) ->
+  st_pc st = (block_entry le) ->
+  exists st',
+    plus (step g) st st' /\
+    st_pc st' = (block_entry lr) /\
+    st_mem st' = (Memory.update (st_mem st) v (aeval a (st_mem st))).
+*)
+
+(*
+Definition comp_store_correct_checker_inner'
+           (a : aexp) (v: addr) (lr le: lbl) (cs: list uid)
+           (stm: state_with_meta)
+  : Checker :=
+  let st := V.Opsem.mkst (stm_mem stm) (block_entry le) (stm_loc stm)
+                         (stm_ppc stm) (stm_ploc stm) in
+  let stm := mk_st_with_meta
+               (stm_mem stm) (stm_mem_dom stm)
+               (block_entry le)
+               (stm_loc stm) (stm_loc_dom stm)
+               (stm_ppc stm)
+               (stm_ploc stm) (stm_ploc_dom stm) in
+  let '(g, end_pc) :=
+      wrap_code_in_cfg (block_entry le)
+                       (Stmon.steval (comp_store a v lr) cs) [] in
+  match (V.Opsem.eval_once_and_until_pc g st (block_entry lr) 1000) with
+  | inl err => whenFail ("comp_store_correct: " ++ err) false
+  | inr st' =>
+    if (eq_dec_pc (V.Opsem.st_pc st') (block_entry lr)) then
+      let new_dom := (v :: stm_mem_dom stm) in
+      whenFail ("::: cfg is: " ++ show g ++
+                " ::: initial state pc: " ++ show (stm_pc stm) ++
+                " ::: le: " ++ show le ++ 
+                " ::: lr: " ++ show lr ++
+                " ::: store to " ++ show v ++
+                " ::: curr pc: " ++ show (block_entry lr) ++
+                " ::: final memory: " ++
+                show_memory (V.Opsem.st_mem st') new_dom ++
+                " ::: initial memory: " ++
+                show_memory (V.Opsem.st_mem st) new_dom)
+        (memory_on_domain_checker new_dom
+          (V.Opsem.st_mem st')
+          (V.Opsem.Memory.update (V.Opsem.st_mem st) v
+                                 (aeval a (V.Opsem.st_mem st))))
+    else whenFail "comp_store_correct: pc not expected" false
+  end.
+ *)
+
+Definition comp_store_correct_checker_inner
+           (a : aexp) (v: addr) (lr le: lbl) (cs: list uid)
+           (stm: state_with_meta)
+  : Checker :=
+  let st := V.Opsem.mkst (stm_mem stm) (block_entry le) (stm_loc stm)
+                         (stm_ppc stm) (stm_ploc stm) in
+  let '(g, end_pc) :=
+      wrap_code_in_cfg (block_entry le)
+                       (Stmon.steval (comp_store a v lr) cs) [] in
+  match (V.Opsem.eval_once_and_until_pc g st (block_entry lr) 1000) with
+  | inl err => whenFail ("comp_store_correct: " ++ err) false
+  | inr st' =>
+    if (eq_dec_pc (V.Opsem.st_pc st') (block_entry lr)) then
+      let new_dom := (v :: stm_mem_dom stm) in
+      whenFail "comp_store_correct: memories mismatch"
+               (memory_on_domain_checker new_dom
+                 (V.Opsem.st_mem st')
+                 (V.Opsem.Memory.update (V.Opsem.st_mem st) v
+                                        (aeval a (V.Opsem.st_mem st))))
+    else whenFail "comp_store_correct: pc not expected" false
+  end.
+
+Definition comp_store_correct_checker: Checker :=
+  forAll arbitrary (fun (a: aexp) =>
+  forAll arbitrary (fun (v: addr) =>
+  forAll arbitrary (fun (lr: lbl) =>
+  forAll arbitrary (fun (le: lbl) =>
+  forAll arbitrary (fun (cs: list uid) =>
+  forAll arbitrary (fun (stm: state_with_meta) =>
+    comp_store_correct_checker_inner a v lr le cs stm)))))).
+
+(* QuickChick comp_store_correct_checker. *)
+
+
+Definition comp_cond_correct_checker_inner
+           (b: bexp) (cs: list uid) (le l1 l2: lbl)
+           (stm: state_with_meta)
+  : Checker :=
+  let st := V.Opsem.mkst (stm_mem stm) (block_entry le) (stm_loc stm)
+                         (stm_ppc stm) (stm_ploc stm) in
+  let '(g, end_pc) :=
+      wrap_code_in_cfg (block_entry le)
+                       (Stmon.steval (comp_cond b l1 l2) cs) [] in
+  let l := (if beval b (V.Opsem.st_mem st) then l1 else l2) in  
+  match (V.Opsem.eval_until_pc g st (block_entry l) 1000) with
+  | inl err =>
+    whenFail 
+      ("::: cfg is: " ++ show g ++
+       "::: comp_cond_correct: " ++ err ++
+       "::: looking for pc: " ++ show end_pc
+      )
+      false
+  | inr st' =>
+    if (eq_dec_pc (V.Opsem.st_pc st') (block_entry l)) then 
+      whenFail "comp_store_correct: memories mismatch"
+               (memory_on_domain_checker (stm_mem_dom stm)
+                                         (V.Opsem.st_mem st)
+                                         (V.Opsem.st_mem st'))
+    else whenFail "comp_cond_correct: pc not expected" false
+  end.
+
+Definition comp_cond_correct_checker : Checker :=
+  forAll arbitrary (fun (b: bexp) =>
+  forAll arbitrary (fun (le: lbl) =>
+  forAll arbitrary (fun (l1: lbl) =>
+  forAll arbitrary (fun (l2: lbl) =>
+  forAll arbitrary (fun (cs: list uid) =>
+  forAll arbitrary (fun (stm: state_with_meta) =>
+    comp_cond_correct_checker_inner b cs le l1 l2 stm)))))).
+
+(* QuickChick comp_cond_correct_checker. *)
+
+(*
+Inductive match_config : Imp.com -> (cfg * lbl * lbl) -> Prop :=
+  | MC_Skip : forall bs l,
+      match_config SKIP (bs, l, l)
+  | MC_Ass : forall g l l' uid a cs,
+      insns_at_pc g (block_entry l) (steval (comp_store a uid l') cs) ->
+      match_config (CAss uid a) (g, l, l')
+  | MC_Seq : forall g l1 l2 l3 c1 c2,
+      match_config c1 (g, l1, l2) ->
+      match_config c2 (g, l2, l3) ->
+      match_config (CSeq c1 c2) (g, l1, l3)
+  | MC_If : forall g le lr l1 l2 b c1 c2 cs,
+      match_config c1 (g, l1, lr) ->
+      match_config c2 (g, l2, lr) ->
+      insns_at_pc g (block_entry le) (steval (comp_cond b l1 l2) cs) ->
+      match_config (CIf b c1 c2) (g, le, lr)
+  | MC_While : forall g le lb lr b c cs,
+      match_config c (g, lb, le) ->
+      insns_at_pc g (block_entry le) (steval (comp_cond b lb lr) cs) ->
+      match_config (CWhile b c) (g, le, lr).
+*)
+
+(*
+Definition match_config_checker
+           (c: Imp.com) ((g, l1 l2): cfg * lbl * lbl)
+  : Checker :=
+  match c with
+  | SKIP => whenFail "match_config: labels not equal for skip"
+                    (eq_dec_lbl l1 l2)
+  | 
+*)                    
+
+(*
+Inductive match_states (g:cfg) (r:lbl)
+  : (com * Imp.state) -> Opsem.state -> Prop :=
+  match_states_intro : forall c mem st l,
+    match_config c (g, l, r) ->
+    st_pc st = block_entry l ->
+    st_mem st = mem ->
+    match_states g r (c, mem) st.
+
+Lemma transl_sim_step_final :
+  forall g r imp_st imp_st' vmn_st,
+  Imp.step imp_st imp_st' ->
+  match_states g r imp_st vmn_st ->
+  exists vmn_st',
+    (plus (Opsem.step g) vmn_st vmn_st' \/
+     star (Opsem.step g) vmn_st vmn_st' /\ imp_size imp_st' < imp_size imp_st) /\
+    match_states g r imp_st' vmn_st'.
+*)
